Experimenting with another representation of weakenings
Not fully conclusive: I get that A<wk_id> is convertible to A
but A<wk_up r> is no longer convertible to A<upRen_term_term r>.

theories/Weakening.v
@@ -1,62 +1,42 @@
-From Coq Require Import Lia.
+From Coq Require Import Lia ssrbool.
 From LogRel.AutoSubst Require Import core unscoped Ast Extra.
 From LogRel Require Import Utils BasicAst Notations Context Untyped UntypedReduction.
 
 Inductive weakening : Set :=
-  | _wk_empty : weakening
+  | _wk_id : weakening
   | _wk_step (w : weakening) : weakening
   | _wk_up (w : weakening) : weakening.
-
-Fixpoint _wk_id (Γ : context) : weakening :=
-  match Γ with
-    | nil => _wk_empty
-    | cons _ Γ' => _wk_up (_wk_id Γ')
-  end.
 
 (* Transforms an (intentional) weakening into a renaming *)
 Fixpoint wk_to_ren (ρ : weakening) : nat -> nat :=
   match ρ with
-    | _wk_empty => id
+    | _wk_id => id
     | _wk_step ρ' => (wk_to_ren ρ') >> S
     | _wk_up ρ' => up_ren (wk_to_ren ρ')
   end.
 
-Lemma wk_to_ren_id Γ : (wk_to_ren (_wk_id Γ)) =1 id.
-Proof.
-  induction Γ.
-  1: reflexivity.
-  intros [] ; cbn.
-  2: rewrite IHΓ.
-  all: reflexivity.
-Qed.
-
 Coercion wk_to_ren : weakening >-> Funclass.
 
+Fixpoint is_canonical_wk (ρ : weakening) {struct ρ} : bool :=
+  match ρ with
+  | _wk_id => true
+  | _wk_up (_wk_id) => false
+  | _wk_up ρ => is_canonical_wk ρ
+  | _wk_step ρ => is_canonical_wk ρ
+  end.
+
 Inductive well_weakening : weakening -> context -> context -> Type :=
-  | well_empty : well_weakening _wk_empty ε ε
+  | well_id {Γ} :  well_weakening _wk_id Γ Γ
   | well_step {Γ Δ : context} (na : aname) (A : term) (ρ : weakening) :
     well_weakening ρ Γ Δ -> well_weakening (_wk_step ρ) (Γ,,vass na A) Δ
   | well_up {Γ Δ : context} (na : aname) (A : term) (ρ : weakening) :
     well_weakening ρ Γ Δ -> well_weakening (_wk_up ρ) (Γ,,vass na (ren_term ρ A)) (Δ,, vass na A).
 
-Lemma well_wk_id (Γ : context) : well_weakening (_wk_id Γ) Γ Γ.
-Proof.
-  induction Γ as [|d].
-  1: econstructor.
-  replace d with (d⟨wk_to_ren (_wk_id Γ)⟩) at 2.
-  all: destruct d as [na A].
-  1: now econstructor.
-  cbn.
-  f_equal.
-  rewrite wk_to_ren_id.
-  now asimpl.
-Qed.
-
 Fixpoint wk_compose (ρ ρ' : weakening) : weakening :=
   match ρ, ρ' with
-    | _wk_empty , _ => ρ'
+    | _wk_id , _ => ρ'
     | _wk_step ν , _ => _wk_step (wk_compose ν ρ')
-    | _wk_up ν, _wk_empty => ρ
+    | _wk_up ν, _wk_id => ρ
     | _wk_up ν, _wk_step ν' => _wk_step (wk_compose ν ν')
     | _wk_up ν, _wk_up ν' => _wk_up (wk_compose ν ν')
   end.
@@ -88,6 +68,7 @@ Proof.
   - eassumption.
   - econstructor. auto.
   - inversion H' as [| | ? ? na' A' ν']; subst ; clear H'.
+    1: econstructor; auto.
     1: now econstructor ; auto.
     asimpl.
     replace (ren_term (ν' >> ν) A') with (ren_term (wk_compose ν ν') A')
@@ -96,24 +77,48 @@ Proof.
 Qed.
 
 #[projections(primitive)]Record wk_well_wk {Γ Δ : context} :=
-  { wk :> weakening ; well_wk :> well_weakening wk Γ Δ}.
+  { wk :> weakening ; well_wk :> well_weakening wk Γ Δ ; can_wk : is_canonical_wk wk }.
 Arguments wk_well_wk : clear implicits.
 Arguments Build_wk_well_wk : clear implicits.
 Notation "Γ ≤ Δ" := (wk_well_wk Γ Δ).
 
-Definition wk_empty : (ε ≤ ε) := {| wk := _wk_empty ; well_wk := well_empty |}.
+Definition wk_empty : (ε ≤ ε) := {| wk := _wk_id ; well_wk := well_id ; can_wk := eq_refl |}.
 
 Definition wk_step {Γ Δ} na A (ρ : Γ ≤ Δ) : (Γ,, vass na A) ≤ Δ :=
-  {| wk := _wk_step ρ ; well_wk := well_step na A ρ ρ |}.
-
-Definition wk_up {Γ Δ} na A (ρ : Γ ≤ Δ) : (Γ,, vass na A⟨wk_to_ren ρ⟩) ≤ (Δ ,, vass na A) :=
-  {| wk := _wk_up ρ ; well_wk := well_up na A ρ ρ |}.
+  {| wk := _wk_step ρ ; well_wk := well_step na A ρ ρ ; can_wk := ρ.(can_wk) |}.
 
 Definition wk_id {Γ} : Γ ≤ Γ :=
-  {| wk := _wk_id Γ ; well_wk := well_wk_id Γ |}.
+  {| wk := _wk_id ; well_wk := well_id ; can_wk := eq_refl |}.
+
+Lemma well_id_ext {Γ Δ} na A : well_weakening _wk_id Γ Δ ->
+  well_weakening _wk_id (Γ ,, vass na A⟨wk_to_ren _wk_id⟩) (Δ ,, vass na A).
+Proof.
+  intro h; inversion h.
+  cbn; asimpl.
+  constructor.
+Qed.
+
+Definition wk_up_aux {Γ Δ} na A (ρ : weakening) :
+  well_weakening ρ Γ Δ ->
+  is_canonical_wk ρ ->
+  (Γ,, vass na A⟨wk_to_ren ρ⟩) ≤ (Δ ,, vass na A) :=
+  match ρ with
+  | _wk_id => fun wellwk _ => 
+    {| wk := _wk_id ; well_wk := well_id_ext na A wellwk ; can_wk := eq_refl |}
+  | _wk_step ρ' => 
+    fun wellwk iscan => 
+    let ρ0 := _wk_step ρ' in  
+    {| wk := _wk_up ρ0 ; well_wk := well_up na A ρ0 wellwk ; can_wk := iscan |}
+  | _wk_up ρ' => 
+    fun wellwk iscan => 
+    let ρ0 := _wk_up ρ' in  
+    {| wk := _wk_up ρ0 ; well_wk := well_up na A ρ0 wellwk ; can_wk := iscan |}
+  end.
+
+Definition wk_up {Γ Δ} na A (ρ : Γ ≤ Δ) : (Γ,, vass na A⟨wk_to_ren ρ⟩) ≤ (Δ ,, vass na A) :=
+  wk_up_aux na A ρ.(wk) ρ.(well_wk) ρ.(can_wk).
 
 #[global] Hint Resolve well_wk : core.
-
 
 #[global] Instance Ren1_wk {Y Z : Type} `(ren : Ren1 (nat -> nat) Y Z) :
   (Ren1 weakening Y Z) := fun ρ t => t⟨wk_to_ren ρ⟩.
@@ -131,50 +136,72 @@ Ltac fold_wk_ren :=
 
 Smpl Add fold_wk_ren : refold.
 
+Lemma can_wk_compose{Γ Γ' Γ'' : context} (ρ : Γ ≤ Γ') (ρ' : Γ' ≤ Γ'') :
+  is_canonical_wk (wk_compose ρ.(wk) ρ'.(wk)).
+Proof.
+  destruct ρ as [ρ ? can], ρ' as [ρ' ? can']; cbn; clear -can can'.
+  induction ρ in can, ρ', can' |- *; cbn; tea.
+  1: auto.
+  destruct ρ'; tea; cbn in *.
+  - apply IHρ; tea. destruct ρ; tea; discriminate.
+  - pose proof (ih := fun h => IHρ h ρ').
+    set (ρ'' := wk_compose _ _) in ih |- *.
+    destruct ρ, ρ'; try discriminate; destruct ρ'' eqn: E; try discriminate.
+    all: now apply ih.
+Qed.
+
 Definition wk_well_wk_compose {Γ Γ' Γ'' : context} (ρ : Γ ≤ Γ') (ρ' : Γ' ≤ Γ'') : Γ ≤ Γ'' :=
-  {| wk := wk_compose ρ.(wk) ρ'.(wk) ; well_wk := well_wk_compose ρ.(well_wk) ρ'.(well_wk) |}.
+  {| wk := wk_compose ρ.(wk) ρ'.(wk) ;
+     well_wk := well_wk_compose ρ.(well_wk) ρ'.(well_wk) ; can_wk := can_wk_compose ρ ρ' |}.
 Notation "ρ ∘w ρ'" := (wk_well_wk_compose ρ ρ').
 
 Lemma well_length {Γ Δ : context} (ρ : Γ ≤ Δ) : #|Δ| <= #|Γ|.
 Proof.
-  destruct ρ as [ρ wellρ].
+  destruct ρ as [ρ wellρ _].
   induction wellρ.
   all: cbn ; lia.
+Qed.
+
+Definition wk_id_conv {Γ} : wk_to_ren (@wk_id Γ) = id := eq_refl.
+
+Lemma is_canonical_wk_up ρ : 
+  is_canonical_wk (_wk_up ρ) -> is_canonical_wk ρ.
+Proof.
+  destruct ρ; cbn; try discriminate + trivial.
 Qed.
 
 (* Testing that the definitions are right *)
 Lemma id_ren (Γ : context) (ρ : Γ ≤ Γ) : ρ =1 id.
 Proof.
-  destruct ρ as [ρ wellρ].
+  destruct ρ as [ρ wellρ canρ].
   cbn in *.
   pose proof (@eq_refl _ #|Γ|) as eΓ.
   revert eΓ wellρ.
   generalize Γ at 2 4.
   intros Δ e wellρ.
-  induction wellρ in e |- *.
+  induction wellρ in e, canρ |- *.
   all: cbn.
   - reflexivity.
-  - pose proof (well_length {| wk := ρ ; well_wk := wellρ |}).
+  - pose proof (well_length {| wk := ρ ; well_wk := wellρ ; can_wk := canρ|}).
     now cbn in * ; lia.
   - asimpl.
     setoid_rewrite IHwellρ.
-    2: now cbn in * ; lia.
-    now intros [] ; reflexivity.
+    + now intros [] ; reflexivity.
+    + now apply is_canonical_wk_up. 
+    + now cbn in * ; lia.
 Qed.
 
 
 Definition wk1 {Γ} nA A : Γ,, vass nA A ≤ Γ := wk_step nA A (wk_id (Γ := Γ)).
 
 Lemma wk1_ren {Γ nA A} : @wk1 Γ nA A =1 ↑.
-Proof.
-  intros ?; cbv -[wk_to_ren _wk_id]. cbn. 
-  rewrite (id_ren Γ (@wk_id Γ)). reflexivity.
-Qed.
+Proof. reflexivity. Qed.
 
 Lemma wk_up_ren {Γ Δ nA A} (ρ : Δ ≤ Γ) : 
   wk_up nA A ρ =1 upRen_term_term  ρ.
 Proof.
-  intros; cbn; now asimpl.
+  intros; cbn; asimpl.
+  destruct ρ as [[] ??]; cbn; now intros [].
 Qed.
 
 Lemma map_decl_lift (ρ : weakening) d :
@@ -193,14 +220,14 @@ Lemma in_ctx_wk (Γ Δ : context) n decl (ρ : Δ ≤ Γ) :
   in_ctx Δ (ρ n) (map_decl (ren_term ρ) decl).
 Proof.
   intros Hdecl.
-  destruct ρ as [ρ wfρ] ; cbn.
+  destruct ρ as [ρ wfρ canρ] ; cbn. clear canρ.
   induction wfρ in n, decl, Hdecl |- *.
   - cbn.
     rewrite map_decl_id.
     1: eassumption.
     now asimpl.
   - cbn.
-    change ((ρ >> S) n) with (S (ρ n)).
+    change ((?ρ >> S) n) with (S (ρ n)).
     replace (map_decl _ _) with (map_decl (ren_term shift) (map_decl (ren_term ρ) decl))
       by (now rewrite compose_map_decl ; asimpl).
     now econstructor.
@@ -243,6 +270,31 @@ End RenWlWhnf.
 
 #[global] Hint Resolve whne_ren_wl whnf_ren_wl isType_ren_wl isFun_ren_wl : gen_typing.
 
+Lemma wk_id_ren_on Γ (H : term) : H⟨@wk_id Γ⟩ = H.
+Proof. cbv -[ren_term]; now asimpl. Qed.
+
+
+Lemma wk1_ren_on Γ nF F (H : term) : H⟨@wk1 Γ nF F⟩ = H⟨↑⟩.
+Proof. reflexivity. Qed.
+  
+Lemma wk_up_ren_on Γ Δ (ρ : Γ ≤ Δ) nF F (H : term) : H⟨wk_up nF F ρ⟩ = H⟨upRen_term_term ρ⟩.
+Proof. now rewrite <- (@wk_up_ren _ _ nF F ρ). Qed.
+
+Lemma wk_up_wk1_ren_on Γ nF F nG G (H : term) : H⟨wk_up nF F (@wk1 Γ nG G)⟩ = H⟨upRen_term_term ↑⟩.
+Proof. reflexivity. Qed.
+
+Lemma prod_wk {Γ Δ na dom cod} {ρ : Γ ≤ Δ} : tProd na dom⟨ρ⟩ cod⟨wk_up na dom ρ⟩ = (tProd na dom cod)⟨ρ⟩.
+Proof.  now rewrite wk_up_ren_on. Qed.
+
+Lemma arr_wk {Γ Δ A B} (ρ : Γ ≤ Δ) : arr A⟨ρ⟩ B⟨ρ⟩ = (arr A B)⟨ρ⟩.
+Proof.  cbn; now asimpl. Qed.
+
+Lemma app_eta_wk {Γ Δ nA A f} (ρ : Γ ≤ Δ) :
+ tApp f⟨ρ⟩⟨shift⟩ (tRel 0) = (tApp f⟨shift⟩ (tRel 0))⟨wk_up nA A ρ⟩.
+Proof.
+  cbn; asimpl; rewrite wk_up_ren; now asimpl.
+Qed.
+
 (* Adaptation of Autosubst asimpl to well typed weakenings *)
 Ltac bsimpl' := repeat (first
                  [ progress setoid_rewrite substSubst_term_pointwise
@@ -261,11 +313,11 @@ Ltac bsimpl' := repeat (first
                  | progress setoid_rewrite rinstId'_term
                  | progress setoid_rewrite instId'_term_pointwise
                  | progress setoid_rewrite instId'_term
-                 | progress setoid_rewrite wk_to_ren_id
                  | progress setoid_rewrite wk_compose_compose
                  | progress setoid_rewrite id_ren
                  | progress setoid_rewrite wk1_ren
-                 | progress unfold up_term_term, upRen_term_term, up_ren, wk_well_wk_compose, wk_id, wk_step, wk_up, wk_empty (**, _wk_up, _wk_step *)
+                 | progress setoid_rewrite wk_up_ren
+                 | progress unfold up_term_term, upRen_term_term, up_ren, wk_well_wk_compose, wk_id, wk_step, wk_up, wk_empty 
                  | progress cbn[subst_term ren_term wk wk_to_ren]
                  | progress fsimpl ]).
 
